---
title: "DATA 605 - Discussion 3"
author: "Joshua Sturm"
date: "02/13/2018"
output:
  html_document:
    highlight: pygments
    theme: cerulean
    code_folding: show
    toc: yes
    toc_float: yes
    smart: no
  pdf_document:
    keep_tex: yes
always_allow_html: yes
---

```{r setup, include=FALSE}
knitr::opts_chunk$set(echo = T, warning = F, message = F)
```

Page 419, Exercise T17

## Suppose that $B$ is a nonsingular matrix. Prove that $AB$ is similar to $BA$.

Since $B$ is nonsingular, then it's invertible (Theorem CINM, page 200).\
By Theorem MIMI (page 203), $(B^{-1})^{-1} = B$.\
By Definition MI (page 194), $B^{-1}B = I$.\
By Theorem MMIM (page 182), $BI = B$.

Taking this all together, $(B^{-1})^{-1}AB(B^{-1}) = BA = AB$.

